
\subsection*{Theory}

\begin{enumerate}
\item First 
  \begin{align*}
    \dive a \mathbf b 
    = \dd{}{x_i} \unitV{i} \cdot a b_j \unitV{j} = \dd{ab_j}{x_i} \delta_{ij} 
    = \dd{a}{x_i} b_i + a \dd{b_i}{x_i} 
    = \grad a \cdot \mathbf b + a \dive \mathbf b
  \end{align*}
  then 
  \begin{align*}
    \int_\vol \dive a \mathbf b dV &= \int_\vol \left(\grad a \cdot
      \mathbf b + a \dive \mathbf b\right) dV &\Rightarrow& \int_\srf
    a \mathbf b \cdot \nrmV dS &= \int_\vol \left(\grad a \cdot
      \mathbf b + a \dive \mathbf b\right) dV
  \end{align*}
\item Developing the equation using indices we find
  \begin{align*}
    \dive \aVelV \cdot \shearStressT  
    &= \dd{}{x_i} \unitV{i} \cdot \left(\aVel_i \shearStress_{ij} \unitV{j}\right) 
    = \dd{\aVel_i}{x_j} \shearStress_{ij} + 
    \aVel_i \dd{\shearStress_{ij}}{x_j} = \left(\grad \aVel\right)_{ij} \shearStress_{ij} + 
    \aVel_i \left(\dive \shearStress \right)_i = \grad \aVelV : \shearStressT + 
    \aVelV \cdot \dive \shearStressT    
  \end{align*}
\item We have $\grad \aVelV = \shearRateT + \rotRateT$. Since
  $\shearStressT$ is symmetric and $\rotRateT$ antisymmetric we have
  $\shearStressT:\rotRateT = 0$

  
  Then we replace $\shearStressT = 2 \dynVisc \shearRateT - \lambda
  (\dive \aVelV) \identityT$.
  \begin{align*}
    \shearStressT : \grad \aVelV &= \shearStressT : \shearRateT =
    \left(2 \dynVisc \shearRateT - \bulkVisc \left(\dive \aVelV\right)~
      \identityT\right) : \shearRateT 
  \end{align*}
  
  We have $\identityT : \shearRateT = \shearRate_{ij} \delta_{ij} =
  \sum_i \shearRate_{ii} = \dive \velV$. Then, considering $\bulkVisc
  = 2 \dynVisc / 3$
  \begin{align*}
    \shearStressT : \grad \aVelV 
    &= \shearStressT : \shearRateT 
    = 2 \dynVisc \left(
      \shearRateT:\shearRateT - 
      \frac{1}{3} \left(\dive \aVelV\right)^2 \right)
    = 2 \dynVisc \left(
      \underbrace{\sum_{i\neq j} \shearRate_{ij}^2}_{A} + 
      \underbrace{
        \sum_i \shearRate_{ii}^2 - 
        \frac{1}{3} \sum_i \sum_j \shearRate_{ii} \shearRate_{jj}}_{B}\right) 
  \end{align*}
  
  Since obviously $A \geq 0$, we continue with $B$
  \begin{align*}
    3~B &= 
    2 \shearRate_{11}^2 + 
    2 \shearRate_{22}^2 + 
    2 \shearRate_{33}^2 -  
    2 \shearRate_{11} \shearRate_{22} -
    2 \shearRate_{22} \shearRate_{33} - 
    2 \shearRate_{33} \shearRate_{11} \\
    &=(\shearRate_{11} - \shearRate_{22})^2 +
      (\shearRate_{22} - \shearRate_{33})^2 +
      (\shearRate_{33} - \shearRate_{11})^2 \geq 0
  \end{align*}
  
\item prove
  $\rotV \times \rotV \times \xyzV = - \rot^2 r
  \unitV{r}$
  
\item solid body rotation 

  Without loss of generality, align $\rotV$ with the axis $\unitV{z}$,
  and center it in the origin. Then the equations for a point $\xyzV =
  (x_1,x_2,x_3)$ reduce to
  \begin{align*}
    \ddtM{x_1} &= - \rot x_2 &
    \ddtM{x_2} &= \rot x_1 &
    \ddtM{x_3} &= 0
  \end{align*}
  which has the solution 
  \begin{align*}
    x_1 &= r \cos {\rot t} &
    x_2 &= r \sin {\rot t} &
    x_3 &= C
  \end{align*}
    
\end{enumerate}
